Get first simulation proofs to run

java/v2/gol_simulationScript.sml
@@ -21,9 +21,46 @@ End
 
 (* minor definitions *)
 
-Definition sort_def:
-  sort xs = QSORT (λ((i:int,j:int),_) ((i',j'),_). i < i' ∨ (i = i' ∧ j < j')) xs
+Definition ii_lt_def:
+  ii_lt (i:int,j:int) (i',j') ⇔ i < i' ∨ (i = i' ∧ j < j')
 End
+
+Theorem ii_lt_trans:
+  ii_lt x y ∧ ii_lt y z ⇒ ii_lt x z
+Proof
+  PairCases_on ‘x’
+  \\ PairCases_on ‘y’
+  \\ PairCases_on ‘z’
+  \\ fs [ii_lt_def]
+  \\ intLib.COOPER_TAC
+QED
+
+Theorem SORTED_ii_lt_IMP:
+  SORTED ii_lt xs ⇒ ALL_DISTINCT xs
+Proof
+  Induct_on ‘xs’ \\ fs []
+  \\ Cases_on ‘xs’ \\ fs []
+  \\ PairCases_on ‘h’ \\ PairCases \\ fs []
+  \\ strip_tac \\ gvs []
+  \\ conj_tac
+  >-
+   (rw [] \\ fs []
+    \\ fs [ii_lt_def]
+    \\ intLib.COOPER_TAC)
+  \\ pop_assum mp_tac
+  \\ pop_assum mp_tac
+  \\ qid_spec_tac ‘h0’
+  \\ qid_spec_tac ‘h1’
+  \\ qid_spec_tac ‘t’
+  \\ Induct \\ fs [FORALL_PROD]
+  \\ rpt gen_tac \\ strip_tac \\ strip_tac
+  \\ fs []
+  \\ imp_res_tac ii_lt_trans
+  \\ res_tac \\ fs []
+  \\ rw [] \\ fs []
+  \\ fs [ii_lt_def]
+  \\ intLib.COOPER_TAC
+QED
 
 Definition state_lookup_def:
   state_lookup p xs =
@@ -40,20 +77,78 @@ Definition check_pos_def:
         (state_lookup (i-1,j+1) xs) (state_lookup (i,j+1) xs) (state_lookup (i+1,j+1) xs)
 End
 
-Theorem IMP_step_to_state:
-  (let xs = sort x in
-   let ys = sort y in
-   let xs' = MAP FST xs in
-   let ys' = MAP FST ys in
-   let ps' = influence_of xs' in
-     ALL_DISTINCT xs' ∧
-     ALL_DISTINCT ys' ∧
-     EVERY (λy. MEM y ps') ys' ∧
-     EVERY (check_pos xs ys) ps')
-  ⇒
-  step (to_state x) = to_state y
+Triviality imp_set_eq:
+  s ⊆ p ∧ t ⊆ p ∧ (∀x. x ∈ p ⇒ (x ∈ s ⇔ x ∈ t)) ⇒ s = t
 Proof
-  cheat
+  fs [EXTENSION,SUBSET_DEF] \\ metis_tac []
+QED
+
+Triviality state_lookup_to_state:
+  ALL_DISTINCT (MAP FST xs) ⇒ state_lookup p xs = to_state xs p
+Proof
+  PairCases_on ‘p’
+  \\ fs [state_lookup_def,to_state_def]
+  \\ Cases_on ‘ALOOKUP xs (p0,p1)’ \\ gvs []
+  \\ imp_res_tac ALOOKUP_NONE \\ fs [MEM_MAP]
+  \\ imp_res_tac ALOOKUP_MEM \\ rw []
+  \\ eq_tac \\ rw [] \\ fs []
+  \\ imp_res_tac alistTheory.ALOOKUP_ALL_DISTINCT_MEM
+  \\ fs []
+QED
+
+Definition check_infl_def:
+  check_infl [] ps = T ∧
+  check_infl ((x:int,y:int)::xs) ps =
+    (MEM (x-1,y-1) ps ∧ MEM (x,y-1) ps ∧ MEM (x+1,y-1) ps ∧
+     MEM (x-1,y  ) ps ∧ MEM (x,y  ) ps ∧ MEM (x+1,y  ) ps ∧
+     MEM (x-1,y+1) ps ∧ MEM (x,y+1) ps ∧ MEM (x+1,y+1) ps ∧
+     check_infl xs ps)
+End
+
+Theorem check_infl:
+  check_infl xs ps ⇒ infl (set xs) SUBSET set ps
+Proof
+  Induct_on ‘xs’ \\ fs [check_infl_def]
+  >-
+   (fs [SUBSET_DEF,IN_DEF,infl_def,FORALL_PROD]
+    \\ fs [live_adj_def])
+  \\ fs [SUBSET_DEF,IN_DEF,infl_thm,FORALL_PROD,check_infl_def]
+  \\ rw [] \\ fs []
+  \\ gvs [int_arithTheory.elim_minus_ones]
+QED
+
+Theorem IMP_step_to_state:
+  ∀xs ys ps.
+    (let xs' = MAP FST xs in
+     let ys' = MAP FST ys in
+       ALL_DISTINCT xs' ∧
+       ALL_DISTINCT ys' ∧
+       EVERY (λy. MEM y ps) ys' ∧
+       check_infl xs' ps ∧
+       EVERY (check_pos xs ys) ps)
+    ⇒
+    step (to_state xs) = to_state ys
+Proof
+  rw [] \\ fs [step_def]
+  \\ irule imp_set_eq
+  \\ qexists_tac ‘set ps’
+  \\ ‘step (to_state xs) ⊆ set ps’ by
+   (irule SUBSET_TRANS
+    \\ irule_at Any check_infl
+    \\ first_x_assum $ irule_at Any
+    \\ irule SUBSET_TRANS
+    \\ irule_at Any step_SUBSET_infl
+    \\ irule infl_mono
+    \\ fs [to_state_def,SUBSET_DEF,MEM_MAP,EXISTS_PROD,FORALL_PROD]
+    \\ rw [] \\ pop_assum $ irule_at Any)
+  \\ ‘to_state ys ⊆ set ps’ by
+   (fs [SUBSET_DEF] \\ rw [] \\ PairCases_on ‘x’
+    \\ fs [to_state_def,EVERY_MEM,MEM_MAP,EXISTS_PROD,PULL_EXISTS]
+    \\ res_tac \\ fs [])
+  \\ fs [] \\ PairCases \\ rw []
+  \\ simp [IN_step] \\ fs [EVERY_MEM]
+  \\ first_x_assum drule
+  \\ fs [check_pos_def,gol_def,live_adj_def,IN_DEF,state_lookup_to_state]
 QED
 
 val _ = export_theory();
