java/v2/gol_wiresScript.sml
@@ -1,6 +1,8 @@
-open HolKernel Parse boolLib bossLib;
+open preamble gol_simulationTheory;
 
 val _ = new_theory "gol_wires";
+
+val _ = (max_print_depth := 0);
 
 fun read_file filename = let
   val f = TextIO.openIn filename
@@ -37,16 +39,81 @@ fun parse_line l = let
   in ((x,y),tm) end
 val data = map (map parse_line) ps
 
-val d = hd data
+val (d1::d2::_) = data
 
+val _ = (max_print_depth := 500);
+
+fun prove_all_distinct goal =
+  prove(goal,
+    (irule SORTED_ii_lt_IMP
+     \\ fs [sortingTheory.SORTED_DEF]
+     \\ EVAL_TAC) ORELSE EVAL_TAC)
+
+fun prove_step_to_state d1 d2 = let
   fun mk_int i = intSyntax.term_of_int (Arbint.fromInt i)
   fun mk_pair f g (x,y) = pairSyntax.mk_pair(f x, g y)
   fun mk_iib_list xs = listSyntax.mk_list(xs,“:(int # int) # bool”)
-
+  fun mk_ii_list xs = listSyntax.mk_list(xs,“:int # int”)
+  fun infl [] = []
+    | infl ((x,y)::xs) =
+       (x-1,y-1) :: (x,y-1) :: (x+1,y-1) ::
+       (x-1,y  ) :: (x,y  ) :: (x+1,y  ) ::
+       (x-1,y+1) :: (x,y+1) :: (x+1,y+1) ::  infl xs
+  fun remove_dups [] = []
+    | remove_dups [x] = [x]
+    | remove_dups (x::y::ys) =
+        if x = y then remove_dups (x::ys) else x :: remove_dups (y::ys)
+  val ps = infl (d1 |> map fst)
+           |> sort (fn (i,j) => fn (i',j') => (i < i') orelse ((i = i') andalso (j < j')))
+           |> remove_dups
+  val xs_tm = map (mk_pair (mk_pair mk_int mk_int) I) d1 |> mk_iib_list
+  val ys_tm = map (mk_pair (mk_pair mk_int mk_int) I) d2 |> mk_iib_list
+  val ps_tm = map (mk_pair mk_int mk_int) ps |> mk_ii_list
+  val th = SPECL [xs_tm,ys_tm,ps_tm] IMP_step_to_state
+           |> PURE_REWRITE_RULE [MAP,FST]
+           |> CONV_RULE (PATH_CONV "lr" (REWR_CONV LET_THM THENC BETA_CONV))
+           |> CONV_RULE (PATH_CONV "lr" (REWR_CONV LET_THM THENC BETA_CONV))
+  val goal = th |> concl |> dest_imp |> fst
+  val (dist_goal1,goal) = dest_conj goal
+  val (dist_goal2,goal) = dest_conj goal
+  val (every_mem_goal,goal) = dest_conj goal
+  val (infl_goal,check_pos_goal) = dest_conj goal
+  val _ = print " - Proving ALL_DISINCT\n"
+  val dist_thm1 = prove_all_distinct dist_goal1
+  val dist_thm2 = prove_all_distinct dist_goal2
+  val _ = print " - Proving EVERY_MEM\n"
+  val every_mem_thm = prove_all_distinct every_mem_goal
+  val _ = print " - Proving check_infl\n"
+  val check_infl_thm = prove_all_distinct infl_goal
+  val _ = print " - Proving check_pos\n"
+  fun case_all_goal_vars_tac (asms,goal) = let
+    val vs = free_vars goal
+    fun tac [] = all_tac
+      | tac (v::vs) = tmCases_on v [] THEN tac vs
+    in tac vs (asms,goal) end
 (*
-
-  map (mk_pair (mk_pair mk_int mk_int) I) d |> mk_iib_list
-
+    set_goal([],check_pos_goal)
 *)
+  val check_pos_thm = prove(check_pos_goal,
+    rpt (once_rewrite_tac [EVERY_DEF]
+         \\ conj_tac >- (EVAL_TAC \\ rewrite_tac [gol_simTheory.gol_simp]
+                         \\ case_all_goal_vars_tac
+                         \\ rewrite_tac [gol_simTheory.gol_simp]))
+    \\ rewrite_tac [EVERY_DEF])
+  val _ = print " - Composing all lemmas\n"
+  val lemma =
+    LIST_CONJ [dist_thm1,dist_thm2,every_mem_thm,check_infl_thm,check_pos_thm]
+  in MP th lemma end
+
+fun prove_all_steps data = let
+  fun prove_steps i [] = []
+    | prove_steps i [d] = []
+    | prove_steps i (d1::d2::ds) = let
+    val _ = print ("Step " ^ int_to_string i ^ ":\n")
+    val th = prove_step_to_state d1 d2
+    in th :: prove_steps (i+1) (d2::ds) end
+  in prove_steps 1 data end
+
+val thms = time prove_all_steps (curry List.take data 3);
 
 val _ = export_theory();
